% \begin{aligned}
%     \tan x & =\sum_{n=0}^{\infty} \frac{U_{2 n+1}}{(2 n+1) !} x^{2 n+1} \\
%     & =\sum_{n=1}^{\infty} \frac{(-1)^{n-1} 2^{2 n}\left(2^{2 n}-1\right) B_{2 n}}{(2 n) !} x^{2 n-1} \\
%     & =x+\frac{1}{3} x^3+\frac{2}{15} x^5+\frac{17}{315} x^7+\cdots, \quad \text { for }|x|<\frac{\pi}{2} . \\
%     \csc x & =\sum_{n=0}^{\infty} \frac{(-1)^{n+1} 2\left(2^{2 n-1}-1\right) B_{2 n}}{(2 n) !} x^{2 n-1} \\
%     & =x^{-1}+\frac{1}{6} x+\frac{7}{360} x^3+\frac{31}{15120} x^5+\cdots, \quad \text { for } 0<|x|<\pi . \\
%     \sec x & =\sum_{n=0}^{\infty} \frac{U_{2 n}}{(2 n) !} x^{2 n}=\sum_{n=0}^{\infty} \frac{(-1)^n E_{2 n}}{(2 n) !} x^{2 n} \\
%     & =1+\frac{1}{2} x^2+\frac{5}{24} x^4+\frac{61}{720} x^6+\cdots, \quad \text { for }|x|<\frac{\pi}{2} . \\
%     \cot x & =\sum_{n=0}^{\infty} \frac{(-1)^n 2^{2 n} B_{2 n}}{(2 n) !} x^{2 n-1} \\
%     & =x^{-1}-\frac{1}{3} x-\frac{1}{45} x^3-\frac{2}{945} x^5-\cdots, \quad \text { for } 0<|x|<\pi .
% \end{aligned}


$$
\begin{aligned}
\tan x & =\sum_{n=0}^{\infty} \frac{U_{2 n+1}}{(2 n+1) !} x^{2 n+1} \\
& =\sum_{n=1}^{\infty} \frac{(-1)^{n-1} 2^{2 n}\left(2^{2 n}-1\right) B_{2 n}}{(2 n) !} x^{2 n-1} \\
& =x+\frac{1}{3} x^3+\frac{2}{15} x^5+\frac{17}{315} x^7+\cdots, \quad \text { for }|x|<\frac{\pi}{2} . \\
\csc x & =\sum_{n=0}^{\infty} \frac{(-1)^{n+1} 2\left(2^{2 n-1}-1\right) B_{2 n}}{(2 n) !} x^{2 n-1} \\
& =x^{-1}+\frac{1}{6} x+\frac{7}{360} x^3+\frac{31}{15120} x^5+\cdots, \quad \text { for } 0<|x|<\pi . \\
\sec x & =\sum_{n=0}^{\infty} \frac{U_{2 n}}{(2 n) !} x^{2 n}=\sum_{n=0}^{\infty} \frac{(-1)^n E_{2 n}}{(2 n) !} x^{2 n} \\
& =1+\frac{1}{2} x^2+\frac{5}{24} x^4+\frac{61}{720} x^6+\cdots, \quad \text { for }|x|<\frac{\pi}{2} . \\
\cot x & =\sum_{n=0}^{\infty} \frac{(-1)^n 2^{2 n} B_{2 n}}{(2 n) !} x^{2 n-1} \\
& =x^{-1}-\frac{1}{3} x-\frac{1}{45} x^3-\frac{2}{945} x^5-\cdots, \quad \text { for } 0<|x|<\pi .
\end{aligned}
$$